HybridVerifVecs/funcsets/cat2funcset_examples.thy
@@ -229,7 +229,7 @@ abbreviation circular_motion_matrix :: "real^2^2"
 notation circular_motion_matrix ("C")
 
 lemma circle_invariant: 
-  "(\<lambda>s. r\<^sup>2 = (s $ 0)\<^sup>2 + (s $ 1)\<^sup>2) is_diff_invariant_of (*v) C along UNIV UNIV from 0"
+  "diff_invariant (\<lambda>s. r\<^sup>2 = (s $ 0)\<^sup>2 + (s $ 1)\<^sup>2) ((*v) C) UNIV UNIV 0 G"
   apply(rule_tac diff_invariant_rules, clarsimp, simp, clarsimp)
   apply(frule_tac i="0" in has_vderiv_on_vec_nth, drule_tac i="1" in has_vderiv_on_vec_nth)
   apply(rule_tac S="UNIV" in has_vderiv_on_subset)
@@ -237,8 +237,7 @@ lemma circle_invariant:
 
 lemma circular_motion_invariants:
   "{s. r\<^sup>2 = (s $ 0)\<^sup>2 + (s $ 1)\<^sup>2} \<le> fb\<^sub>\<F> (x\<acute>=(*v) C & G) {s. r\<^sup>2 = (s $ 0)\<^sup>2 + (s $ 1)\<^sup>2}"
-  apply(rule_tac I="\<lambda>s. r\<^sup>2 = (s $ 0)\<^sup>2 + (s $ 1)\<^sup>2" in dInvariant)
-  using circle_invariant by auto
+  unfolding dInvariant using circle_invariant by auto
 
 \<comment> \<open>Proof of the same specification by providing solutions:\<close>
 
@@ -355,14 +354,14 @@ subsubsection\<open> Bouncing Ball with invariants \<close>
 
 text\<open> We prove again the bouncing ball but this time with differential invariants. \<close>
 
-lemma gravity_invariant: "(\<lambda>s. s $ 2 < 0) is_diff_invariant_of (*v) A along UNIV UNIV from 0"
+lemma gravity_invariant: "diff_invariant (\<lambda>s. s $ 2 < 0) ((*v) A) UNIV UNIV 0 G"
   apply(rule_tac \<theta>'="\<lambda>s. 0" and \<nu>'="\<lambda>s. 0" in diff_invariant_rules(3), clarsimp, simp, clarsimp)
   apply(drule_tac i="2" in has_vderiv_on_vec_nth)
   apply(rule_tac S="UNIV" in has_vderiv_on_subset)
   by(auto intro!: poly_derivatives simp: vec_eq_iff matrix_vector_mult_def)
 
 lemma energy_conservation_invariant: 
-  "(\<lambda>s. 2 \<cdot> s$2 \<cdot> s$0 - 2 \<cdot> s$2 \<cdot> h - s$1 \<cdot> s $ 1 = 0) is_diff_invariant_of (*v) A along UNIV UNIV from 0"
+  "diff_invariant (\<lambda>s. 2 \<cdot> s$2 \<cdot> s$0 - 2 \<cdot> s$2 \<cdot> h - s$1 \<cdot> s $ 1 = 0) ((*v) A) UNIV UNIV 0 G"
   apply(rule diff_invariant_rules, simp, simp, clarify)
   apply(frule_tac i="2" in has_vderiv_on_vec_nth)
   apply(frule_tac i="1" in has_vderiv_on_vec_nth)
@@ -373,19 +372,19 @@ lemma energy_conservation_invariant:
 lemma bouncing_ball_invariants:
   fixes h::real
   defines dinv: "I \<equiv> \<lambda>s::real^3. s $ 2 < 0 \<and> 2 \<cdot> s$2 \<cdot> s$0 - 2 \<cdot> s$2 \<cdot> h - (s$1 \<cdot> s$1) = 0"
-  shows "{s\<in>UNIV. 0 \<le> s $ 0 \<and> s $ 0 = h \<and> s $ 1 = 0 \<and> 0 > s $ 2} \<le> fb\<^sub>\<F> 
-  (kstar ((x\<acute>=(*v) A & (\<lambda> s. s $ 0 \<ge> 0) on UNIV UNIV @ 0) \<circ>\<^sub>K
+  shows "{s. 0 \<le> s $ 0 \<and> s $ 0 = h \<and> s $ 1 = 0 \<and> 0 > s $ 2} \<le> 
+  fb\<^sub>\<F> (kstar ((x\<acute>=(*v) A & (\<lambda> s. s $ 0 \<ge> 0)) \<circ>\<^sub>K
   (IF (\<lambda> s. s $ 0 = 0) THEN (1 ::= (\<lambda>s. - s $ 1)) ELSE \<eta> FI)))
-  {s\<in>UNIV. 0 \<le> s $ 0 \<and> s $ 0 \<le> h}"
-  apply(rule_tac I="{s\<in>UNIV. 0 \<le> s$0 \<and> I s}" in ffb_kstarI)
+  {s. 0 \<le> s $ 0 \<and> s $ 0 \<le> h}"
+  apply(rule_tac I="{s. 0 \<le> s$0 \<and> I s}" in ffb_kstarI)
   apply(force simp: dinv, simp only: ffb_kcomp)
-   apply(rule_tac I="{s\<in>UNIV. 0 \<le> s$0 \<and> I s}" in dI)
+   apply(rule_tac I="{s. 0 \<le> s$0 \<and> I s}" in dI)
   apply(simp_all, subst ffb_guard_eq, simp)
     apply(rule_tac y="{s. I s}" in H_iso_cond1, force)
-  apply(rule dInvariant[of I], unfold dinv)
+    apply(unfold dInvariant dinv)
     apply(intro diff_invariant_rules(4))
   using gravity_invariant apply force
-  using energy_conservation_invariant apply(force, force)
+  using energy_conservation_invariant apply force
    apply(subst ffb_if_then_else)
   unfolding dinv by(auto simp: bb_real_arith le_fun_def)
 
@@ -479,7 +478,7 @@ lemma bouncing_ball_K:
    apply(subst local_flow.ffb_g_orbit[OF local_flow_exp], simp, clarify)
    apply(rule ffb_if_then_elseI, clarsimp)
    apply(simp_all add: sq_mtx_vec_prod_eq)
-  unfolding UNIV_3 apply(simp_all add: exp_cnst_acc_sq_mtx_simps)
+  unfolding UNIV_3 image_le_pred apply(simp_all add: exp_cnst_acc_sq_mtx_simps)
   subgoal for x using bb_real_arith(3)[of "x $ 2"]
     by (simp add: add.commute mult.commute)
   subgoal for x \<tau> using bb_real_arith(4)[where g="x $ 2" and v="x $ 1"]
@@ -487,5 +486,77 @@ lemma bouncing_ball_K:
   by (force simp: bb_real_arith)
 
 no_notation constant_acceleration_kinematics_sq_mtx ("K")
+
+(**************************************************************************************************)
+
+lemma 
+  fixes \<tau>::real
+  assumes invH: "2 \<cdot> g \<cdot> x = 2 \<cdot> g \<cdot> h + v \<cdot> v \<or> 
+  (\<exists>n. v\<^sup>2 = 2 \<cdot> g \<cdot> (x - h - h \<cdot> (c\<^sup>2 - 1) \<cdot> (\<Sum>m\<le>n. c ^ (2 \<cdot> m))))"
+    and posH: "g \<cdot> \<tau>\<^sup>2 / 2 + v \<cdot> \<tau> + x = 0"
+  shows "2 \<cdot> g \<cdot> h + c \<cdot> (g \<cdot> \<tau> + v) \<cdot> (c \<cdot> (g \<cdot> \<tau> + v)) = 0 \<or> 
+  (\<exists>n::nat. (c \<cdot> (g \<cdot> \<tau> + v))\<^sup>2 = 2 \<cdot> g \<cdot> (- h - h \<cdot> (c\<^sup>2 - 1) \<cdot> (\<Sum>m\<le>n. c ^ (2 \<cdot> m))))"
+proof(rule disjE[OF invH])
+  assume invH1: "2 \<cdot> g \<cdot> x = 2 \<cdot> g \<cdot> h + v \<cdot> v"
+  define n::nat where n_def: "n \<equiv> 0"
+  note arg_cong[OF posH, of "\<lambda>t. 2 \<cdot> g \<cdot> t"]
+  hence "g\<^sup>2 \<cdot> \<tau>\<^sup>2 + 2 \<cdot> g \<cdot> v \<cdot> \<tau> + 2 \<cdot> g \<cdot> x = 0"
+    by (simp add: distrib_left[of "2 \<cdot> g"] mult_ac(1)[symmetric] power2_eq_square)
+  hence "(g \<cdot> \<tau> + v)\<^sup>2 = - 2 \<cdot> g \<cdot> h"
+    by (simp add: power2_sum[of "g \<cdot> \<tau>" v] field_simps(48) mult_ac(1)[symmetric] invH1 
+        power2_eq_square[symmetric, of v]) (simp add: mult.commute mult_ac(3))
+  hence "c\<^sup>2 \<cdot> (g \<cdot> \<tau> + v)\<^sup>2 = 2 \<cdot> g \<cdot> (- h - h \<cdot> (c\<^sup>2 - 1))"
+    by (simp add: cross3_simps(25) field_simps(48))
+  hence "(c \<cdot> (g \<cdot> \<tau> + v))\<^sup>2 = 2 \<cdot> g \<cdot> (- h - h \<cdot> (c\<^sup>2 - 1) \<cdot> (\<Sum>m\<le>n. c ^ (2 \<cdot> m)))"
+    by (simp add: n_def field_simps(48))
+  thus ?thesis
+    by blast
+next
+  assume "\<exists>n. v\<^sup>2 = 2 \<cdot> g \<cdot> (x - h - h \<cdot> (c\<^sup>2 - 1) \<cdot> (\<Sum>m\<le>n. c ^ (2 \<cdot> m)))"
+  then obtain n where invH2: "v\<^sup>2 = 2 \<cdot> g \<cdot> (x - h - h \<cdot> (c\<^sup>2 - 1) \<cdot> (\<Sum>m\<le>n. c ^ (2 \<cdot> m)))"
+    by blast
+
+thm mult_ac(1,3) mult_minus_left mult_zero_right power2_eq_square distrib_left 
+  mult.commute field_simps(48) cross3_simps(25)
+  oops
+
+notation constant_acceleration_kinematics_matrix ("A")
+
+lemma bouncing_ball:
+  assumes "(h::real) > 0" and "0 < c" and "c < 1"
+  shows "{s. s $ 0 = h \<and> s $ 1 = 0 \<and> 0 > s $ 2} \<le> fb\<^sub>\<F> 
+  (kstar ((x\<acute>=(*v) A & (\<lambda> s. s $ 0 \<ge> 0)) \<circ>\<^sub>K
+  (IF (\<lambda> s. s $ 0 = 0) THEN (1 ::= (\<lambda>s. - c * s $ 1)) ELSE \<eta> FI)))
+  {s. 0 \<le> s $ 0 \<and> s $ 0 \<le> h}"  
+  apply(rule ffb_kstarI[of _ "{s. 0 \<le> s$0 \<and> s$0 \<le> h \<and> 0 > s$2 \<and> 
+  (2 \<cdot> s$2 \<cdot> s$0 = 2 \<cdot> s$2 \<cdot> h + s$1 \<cdot> s$1 \<or> (\<exists>n::nat. s$1^2 = 2 * (s$2) * ((s$0) - h - h * (c^2 - 1) * (\<Sum>m \<le> n. c ^ (2 \<cdot> m)))))}"])
+  using \<open>h > 0\<close> apply force 
+  prefer 2 apply force
+   apply(subst ffb_kcomp)
+  apply(subst local_flow.ffb_g_orbit[OF local_flow_cnst_acc_matrix], simp)
+apply(subst ffb_if_then_else)
+  apply(safe, simp add: )
+  oops
+
+thm continuous_on_cases
+thm vec_tendstoI continuous_on_vec_lambda
+
+lemma bouncing_ball:
+  shows "{s. 0 \<le> s $ 0 \<and> s $ 0 = h \<and> s $ 1 = 0 \<and> 0 > s $ 2} \<le> fb\<^sub>\<F> 
+  (kstar ((x\<acute>=(*v) A & (\<lambda> s. s $ 0 \<ge> 0)) \<circ>\<^sub>K
+  (IF (\<lambda> s. s $ 0 = 0) THEN (1 ::= (\<lambda>s. - s $ 1)) ELSE \<eta> FI)))
+  {s. 0 \<le> s $ 0 \<and> s $ 0 \<le> h}"
+  apply(rule ffb_kstarI[of _ "{s. 0 \<le> s$0 \<and> 0 > s$2 \<and>  2 \<cdot> s$2 \<cdot> s$0 = 2 \<cdot> s$2 \<cdot> h + (s$1 \<cdot> s$1)}"])
+    apply(clarsimp, simp only: ffb_kcomp)
+  prefer 2 apply (force simp: bb_real_arith)
+  apply(subst ffb_g_orbital, subst ffb_if_then_else)
+   apply(simp add: ivp_sols_def, clarsimp)
+   apply(frule_tac i=0 in has_vderiv_on_vec_nth)
+  apply(frule_tac i=1 in has_vderiv_on_vec_nth)
+  apply(drule_tac i=2 in has_vderiv_on_vec_nth)
+   apply(simp add: matrix_vector_mult_def axis_def)
+  oops
+
+no_notation constant_acceleration_kinematics_matrix ("A")
 
 end
