HybridVerifVecs/rels/kat2rel.thy
@@ -89,9 +89,9 @@ abbreviation g_evol ::"(('a::banach)\<Rightarrow>'a) \<Rightarrow> 'a pred \<Rig
 subsection \<open>Verification by providing solutions\<close>
 
 lemma sH_g_evolution: 
-  assumes "\<forall>s. P s \<longrightarrow> (\<forall>x\<in>ivp_sols (\<lambda>t. f) T S t\<^sub>0 s. \<forall>t\<in>T. (G \<rhd> x (down T t)) \<longrightarrow> Q (x t))"
+  assumes "\<forall>s. P s \<longrightarrow> (\<forall>X\<in>ivp_sols (\<lambda>t. f) T S t\<^sub>0 s. \<forall>t\<in>T. (\<P> X (down T t) \<subseteq> {s. G s}) \<longrightarrow> Q (X t))"
   shows "rel_kat.H \<lceil>P\<rceil> (x\<acute>=f & G on T S @ t\<^sub>0) \<lceil>Q\<rceil>"
-  using assms unfolding g_orbital_eq sH_H ivp_sols_def by auto
+  using assms unfolding g_orbital_eq(1) sH_H by auto
 
 lemma sH_guard_rule: 
   assumes "R = (\<lambda>s. G s \<and> Q s)" and "rel_kat.H \<lceil>P\<rceil> (x\<acute>=f & G on T S @ t\<^sub>0) \<lceil>Q\<rceil>" 
@@ -107,9 +107,9 @@ lemma sH_orbit:
   using orbit_eq assms(2) unfolding assms(1) sH_H by auto
 
 lemma sH_g_orbit: 
-  assumes "S = UNIV" and "\<forall>s. P s \<longrightarrow> (\<forall>t\<in>T. (G \<rhd> (\<lambda>t. \<phi> t s) (down T t)) \<longrightarrow> Q (\<phi> t s))"
+  assumes "S = UNIV" and "\<forall>s. P s \<longrightarrow> (\<forall>t\<in>T. (\<P> (\<lambda>t. \<phi> t s) (down T t) \<subseteq> {s. G s}) \<longrightarrow> Q (\<phi> t s))"
   shows "rel_kat.H \<lceil>P\<rceil> (x\<acute>=f & G on T S @ 0) \<lceil>Q\<rceil>"
-  using g_orbit_eq assms(2) unfolding assms(1) by (auto simp: sH_H)
+  using g_orbital_collapses assms(2) unfolding assms(1) by (auto simp: sH_H)
 
 lemma invariant_set_eq_dl_invariant:
   assumes "S = UNIV"
@@ -124,7 +124,7 @@ a version of it as an inference rule. A simple computation of a wlp is shown imm
 
 lemma dSolution:
   assumes "local_flow f T UNIV \<phi>"
-    and "\<forall>s. P s \<longrightarrow> (\<forall> t\<in>T. (G \<rhd> (\<lambda>\<tau>. \<phi> \<tau> s) (down T t)) \<longrightarrow> Q (\<phi> t s))"
+    and "\<forall>s. P s \<longrightarrow> (\<forall> t\<in>T. (\<P> (\<lambda>t. \<phi> t s) (down T t) \<subseteq> {s. G s}) \<longrightarrow> Q (\<phi> t s))"
   shows "rel_kat.H \<lceil>P\<rceil> (x\<acute>=f & G on T UNIV @ 0) \<lceil>Q\<rceil>"
   using assms by(subst local_flow.sH_g_orbit, auto)
 
@@ -138,7 +138,7 @@ lemma line_is_local_flow:
 
 lemma line_DS: fixes c::"'a::{heine_borel, banach}"
   assumes "0 \<in> T" and "is_interval T" "open T"
-    and "\<forall>s. P s \<longrightarrow> (\<forall>t\<in>T. (G \<rhd> (\<lambda>\<tau>. s + \<tau> *\<^sub>R c) (down T t)) \<longrightarrow> Q (s + t *\<^sub>R c))"
+    and "\<forall>s. P s \<longrightarrow> (\<forall>t\<in>T. (\<P> (\<lambda> t. s + t *\<^sub>R c) (down T t) \<subseteq> {s. G s}) \<longrightarrow> Q (s + t *\<^sub>R c))"
   shows "rel_kat.H \<lceil>P\<rceil> (x\<acute>=(\<lambda>s. c) & G on T UNIV @ 0) \<lceil>Q\<rceil>"
   apply(subst local_flow.sH_g_orbit[where f="\<lambda>s. c" and \<phi>="(\<lambda> t x. x + t *\<^sub>R c)"])
   using line_is_local_flow assms by auto
@@ -164,34 +164,24 @@ theorem dCut:
     and wp_C:"rel_kat.H \<lceil>P\<rceil> (x\<acute>=f & G on T S @ t\<^sub>0) \<lceil>C\<rceil>"
     and wp_Q:"rel_kat.H \<lceil>P\<rceil> (x\<acute>=f & (\<lambda> s. G s \<and> C s) on T S @ t\<^sub>0) \<lceil>Q\<rceil>"
   shows "rel_kat.H \<lceil>P\<rceil> (x\<acute>=f & G on T S @ t\<^sub>0) \<lceil>Q\<rceil>"
-proof(subst sH_H, simp add: g_orbital_eq p2r_def, clarsimp)
-  fix \<tau>'::real and x::"real \<Rightarrow> 'a" 
-  assume guard_x:" \<forall>\<tau>. \<tau> \<in> T \<and> \<tau> \<le> \<tau>' \<longrightarrow> G (x \<tau>)" and "\<tau>' \<in> T"
-    and x_solves:"D x = (\<lambda>t. f (x t)) on T" "x \<in> T \<rightarrow> S" and "P (x t\<^sub>0)"
-  hence "\<forall>r\<in>(down T \<tau>'). x r \<in> (g_orbital f G T S t\<^sub>0) (x t\<^sub>0)"
-    by (auto intro!: g_orbitalI x_solves \<open>\<tau>' \<in> T\<close>)
-  hence "\<forall>t\<in>(down T \<tau>'). C (x t)" 
-    using wp_C \<open>P (x t\<^sub>0)\<close> by (subst (asm) sH_H, auto)
-  hence "x \<tau>' \<in> (g_orbital f (\<lambda>s. G s \<and> C s) T S t\<^sub>0) (x t\<^sub>0)"
-    apply(simp) apply(rule g_orbitalI)
-    using guard_x by (auto intro!: x_solves \<open>\<tau>' \<in> T\<close>)
-  thus "Q (x \<tau>')"
-    using \<open>P (x t\<^sub>0)\<close> wp_Q by (subst (asm) sH_H) auto
+proof(subst sH_H, simp add: g_orbital_eq p2r_def image_le_pred, clarsimp)
+  fix t::real and X::"real \<Rightarrow> 'a" and s assume "P s" and "t \<in> T"
+    and x_ivp:"X \<in> ivp_sols (\<lambda>t. f) T S t\<^sub>0 s" 
+    and guard_x:"\<forall>x. x \<in> T \<and> x \<le> t \<longrightarrow> G (X x)"
+  have "\<forall>t\<in>(down T t). X t \<in> g_orbital f G T S t\<^sub>0 s"
+    using g_orbitalI[OF x_ivp] guard_x unfolding image_le_pred by auto
+  hence "\<forall>t\<in>(down T t). C (X t)" 
+    using wp_C \<open>P s\<close> by (subst (asm) sH_H, auto)
+  hence "X t \<in> g_orbital f (\<lambda>s. G s \<and> C s) T S t\<^sub>0 s"
+    using guard_x \<open>t \<in> T\<close> by (auto intro!: g_orbitalI x_ivp)
+  thus "Q (X t)"
+    using \<open>P s\<close> wp_Q by (subst (asm) sH_H) auto
 qed
 
 subsubsection\<open> Differential Invariant \<close>
 
-lemma dInvariant:
-  assumes "I is_diff_invariant_of f along T S from t\<^sub>0" and "I\<^sub>S = (\<lambda>s. s\<in>S \<and> I s)"
-  shows "rel_kat.H \<lceil>I\<^sub>S\<rceil> (x\<acute>=f & G on T S @ t\<^sub>0) \<lceil>I\<^sub>S\<rceil>"
-  apply(rule sH_g_evolution) using assms(1) 
-  by (auto simp: diff_invariant_def ivp_sols_def assms(2))
-
-lemma dInvariant_converse:
-  assumes "rel_kat.H \<lceil>\<lambda>s. s\<in>S \<and> I s\<rceil> (x\<acute>=f & (\<lambda>s. True) on T S @ t\<^sub>0) \<lceil>\<lambda>s. s\<in>S \<and> I s\<rceil>"
-  shows "I is_diff_invariant_of f along T S from t\<^sub>0"
-  using assms unfolding invariant_to_set sH_H apply safe
-  by(erule_tac x=s in allE, erule_tac x=x in allE, simp)
+lemma dInvariant:"rel_kat.H \<lceil>I\<rceil> (x\<acute>=f & G on T S @ t\<^sub>0) \<lceil>I\<rceil> = diff_invariant I f T S t\<^sub>0 G"
+  unfolding diff_invariant_eq sH_H g_orbital_eq by auto
 
 lemma dI:
   assumes Thyp: "is_interval T" "t\<^sub>0 \<in> T"
